TransVal/Guards.v
@@ -75,7 +75,7 @@ simpl; split.
               simpl. eapply IHe2; eauto. rewrite <- H0; eauto.
              * rewrite H in H0; rewrite H1 in H0; simpl in H0;  simpl.
                exfalso; discriminate H0.
-          + destruct b.
+          + simpl in EQ2.
             * case_eq (undef e1); case_eq (undef e2); intros.
               {  rewrite H in H0; rewrite H1 in H0. simpl in H0. inversion H0.
                  unfold binop_eval in EQ2.  clear H0. unfold bvDiv in EQ2.
@@ -84,7 +84,7 @@ simpl; split.
                    + intros.  rewrite H0 in EQ2.  exfalso; discriminate EQ2.
                    + intros A.   unfold evalSexp. intros. clear H3. clear EQ2.
                      hnf in H0.  rewrite EQ1 in H0.  simpl in H0. simpl  in A.
-                     eapply  (not_zero_implies_uneq _ k  A) in H0;  eauto.
+                     eapply  (not_zero_implies_uneq _  A) in H0;  eauto.
                  - split.
                    + eapply IHe1; eauto.
                    + eapply IHe2; eauto.  }
@@ -95,7 +95,7 @@ simpl; split.
                    + intros.  rewrite H0 in EQ2.  exfalso; discriminate EQ2.
                    + intros A.   unfold evalSexp. intros. clear H3. clear EQ2.
                      hnf in H0. rewrite EQ1 in H0.  simpl in H0. simpl  in A.
-                     eapply ( not_zero_implies_uneq _ k) in H0; eauto.
+                     eapply ( not_zero_implies_uneq _) in H0; eauto.
                  -  eapply IHe1; eauto. }
                  { rewrite H in H0; rewrite H1 in H0; simpl in H0. inversion H0.
                    unfold binop_eval in EQ2. clear H0. unfold bvDiv in EQ2.
@@ -104,7 +104,7 @@ simpl; split.
                    + intros.  rewrite H0 in EQ2.  exfalso; discriminate EQ2.
                    + intros A.   unfold evalSexp. intros. clear H3. clear EQ2.
                      hnf in H0.  rewrite EQ1 in H0.  simpl in H0. simpl  in A.
-                     eapply  (not_zero_implies_uneq _ k) in H0; eauto.
+                     eapply  (not_zero_implies_uneq _) in H0; eauto.
                  -  eapply IHe2; eauto. }
                  { rewrite H in H0; rewrite H1 in H0; simpl in H0. inversion H0.
                    unfold binop_eval in EQ2. clear H0.
@@ -113,8 +113,8 @@ simpl; split.
                    - intros.  rewrite H0 in EQ2.  exfalso; discriminate EQ2.
                    - intros A.   unfold evalSexp. intros. clear H3. clear EQ2.
                      hnf in H0. rewrite EQ1 in H0.  simpl in H0. simpl  in A.
-                     eapply  (not_zero_implies_uneq _ k) in H0; eauto.    }
-                 * case_eq (undef e1); case_eq (undef e2); intros; simpl.
+                     eapply  (not_zero_implies_uneq _ ) in H0; eauto. } }
+(*                 * case_eq (undef e1); case_eq (undef e2); intros; simpl.
                    { rewrite H in H0; rewrite H1 in H0; simpl in H0.
                      inversion H0. simpl; split.
                      - eapply IHe1; eauto.
@@ -126,7 +126,7 @@ simpl; split.
                      inversion H0. simpl.
                      - eapply IHe2; eauto. rewrite <- H3. assumption. }
                    {  rewrite H in H0; rewrite H1 in H0; simpl in H0.
-                      inversion H0. } }
+                      inversion H0. } } *)
 Qed.
 
 Lemma guardList_true_if_eval:
@@ -167,15 +167,13 @@ Proof.
          rewrite H2; eauto.
       + exists (neg x); unfold option_lift1.
           destruct u; eauto.
-          admit.
   - specialize (IHe1 E); specialize (IHe2 E). simpl in H. cset_tac.
     assert (forall x, x ∈ Exp.freeVars e1 -> exists v, E x = Some v)
       by (cset_tac; eauto).
     assert (forall x, x ∈ Exp.freeVars e2 -> exists v, E x  = Some v)
       by (cset_tac; eauto).
     specialize (IHe1 H1); specialize (IHe2 H2).
-    destruct b; try destruct b; try destruct b; try destruct b; try destruct b;
-     try destruct b; simpl in *.
+    destructBin b; simpl in *.
     + eapply combine_keep_undef in H0. destruct H0.
       destruct IHe1; destruct IHe2; eauto.
       rewrite H4; rewrite H5. simpl. exists (bvAdd x x0).
@@ -198,7 +196,109 @@ Proof.
       unfold option_lift2; eauto.
     + case_eq (undef e1); case_eq(undef e2); intros;
       rewrite H3 in *; rewrite H4 in *; discriminate H0.
-    + admit.
+(*    + eapply combine_keep_undef in H0; destruct H0.
+      destruct IHe1; destruct IHe2; eauto.
+      rewrite H4, H5; simpl. exists (bvAdd x x0).
+      unfold option_lift2; eauto. *)
+Qed.
+
+Lemma noundef:
+forall E e,
+undef e = None
+-> (forall x, x ∈ Exp.freeVars e -> exists v, E x = Some v)
+-> exists v, exp_eval E e = Some v .
+
+Proof.
+  intros.
+  general induction e; simpl in *.
+  - exists v; eauto.
+  - specialize (H0 v). destruct H0; cset_tac; eauto.
+  - specialize (IHe E H H0). destruct IHe.
+    rewrite H1; simpl. destruct u; simpl; unfold option_lift1.
+  + destruct (val2bool x); eauto.
+  + exists (neg x); eauto.
+- destructBin b; simpl in *.
+  + case_eq(undef e1); case_eq(undef e2); intros;
+    rewrite H1, H2 in H; try isabsurd.
+    destruct (IHe1 E) as [v1 eval1]; eauto; cset_tac; eauto.
+    destruct (IHe2 E) as [v2 eval2]; eauto; cset_tac; eauto.
+    rewrite eval1, eval2; simpl. exists (bvAdd v1 v2); eauto.
+  + case_eq(undef e1); case_eq(undef e2); intros;
+    rewrite H1, H2 in H; try isabsurd.
+    destruct (IHe1 E) as [v1 eval1]; eauto; cset_tac; eauto.
+    destruct (IHe2 E) as [v2 eval2]; eauto; cset_tac; eauto.
+    rewrite eval1, eval2; simpl. exists (bvSub v1 v2); eauto.
+  + case_eq(undef e1); case_eq(undef e2); intros;
+    rewrite H1, H2 in H; try isabsurd.
+    destruct (IHe1 E) as [v1 eval1]; eauto; cset_tac; eauto.
+    destruct (IHe2 E) as [v2 eval2]; eauto; cset_tac; eauto.
+    rewrite eval1, eval2; simpl. exists (bvMult v1 v2); eauto.
+  + case_eq(undef e1); case_eq(undef e2); intros;
+    rewrite H1, H2 in H; try isabsurd.
+    destruct (IHe1 E) as [v1 eval1]; eauto; cset_tac; eauto.
+    destruct (IHe2 E) as [v2 eval2]; eauto; cset_tac; eauto.
+    rewrite eval1, eval2; simpl. exists (bvEq v1 v2); eauto.
+  + case_eq(undef e1); case_eq(undef e2); intros;
+    rewrite H1, H2 in H; try isabsurd.
+    destruct (IHe1 E) as [v1 eval1]; eauto; cset_tac; eauto.
+    destruct (IHe2 E) as [v2 eval2]; eauto; cset_tac; eauto.
+    rewrite eval1, eval2; simpl. exists (neg (bvEq v1 v2)); eauto.
+  + case_eq(undef e1); case_eq(undef e2); intros;
+    rewrite H1, H2 in H; try isabsurd.
+Qed.
+
+Lemma guard_impl_eval:
+forall F E e g,
+ undef e = Some g
+-> models F E g
+-> (forall x, x ∈ Exp.freeVars e -> exists v, E x = Some v)
+-> exists v, exp_eval E e = Some v.
+
+Proof.
+intros. general induction e; try isabsurd; simpl.
+- destruct u; simpl in H.
+  + destruct (IHe F E g H H0) as [v eval]; cset_tac; eauto.
+    rewrite eval. simpl. unfold option_lift1.
+    destruct(val2bool v); eauto.
+ + destruct (IHe F E g H H0) as [v eval]; cset_tac; eauto.
+   rewrite eval; simpl; unfold option_lift1.
+   exists (neg v); eauto.
+- destructBin b; simpl in *.
+  + case_eq (undef e1); case_eq (undef e2); intros; simpl in *;
+    rewrite H2, H3 in H; inversion H.
+    * rewrite <- H5 in H0; simpl in H0.
+      destruct H0.
+      destruct (IHe1 F E s0 H3 H0); cset_tac; eauto.
+      destruct (IHe2 F E s H2 H4); cset_tac; eauto.
+      rewrite H6, H5; simpl. exists (bvAdd x x0); eauto.
+    *  pose proof (noundef E e2 H2).
+       destruct H4; cset_tac; eauto.
+       destruct (IHe1 F E g); cset_tac; eauto.
+       rewrite H4, H5; simpl; unfold option_lift2.
+       exists (bvAdd x0 x); eauto.
+    * admit.
+  + admit.
+  + admit.
+  + admit.
+  + admit.
+  + case_eq (undef e1); case_eq (undef e2); intros; simpl in *;
+    rewrite H2, H3 in H; simpl in H; inversion H;
+    rewrite <- H5 in H0; destruct H0.
+    * clear H5. clear H. simpl in H0. unfold evalSexp in H0; simpl in H0.
+      destruct H4.
+      destruct (IHe1 F E s0); cset_tac; eauto.
+      destruct (IHe2  F E s); cset_tac; eauto.
+      rewrite H5, H6; simpl.
+      rewrite H6 in H0.
+      clear H5. clear H6. clear H1.
+      unfold bvDiv.
+      case_eq (bvZero x0); intros.
+      { eapply (zero_implies_eq x0) in H1. specialize (H0 H1); isabsurd.
+        unfold zext. simpl; eauto. }
+      { eauto. }
+    * admit.
+    * admit.
+    * admit.
 Qed.
 
 (*
