TransVal/tvalTactics.v
@@ -2,6 +2,8 @@ Require Import IL Annotation AutoIndTac Bisim Exp MoreExp Coherence Fresh Util S
 
 Tactic Notation "setSubst" hyp(A) :=hnf in A; simpl in A; cset_tac; eapply A.
 Tactic Notation "setSubst2" hyp(A) := hnf; intros; hnf in A;  eapply A; simpl; cset_tac; eauto.
+Tactic Notation "destructBin" hyp(A) := destruct A; try destruct A;
+                                        try destruct A; try destruct A; try destruct A.
 
 (*
 *** Local Variables: ***
